Phi_Examples/Bucket_Hash.thy
@@ -1,5 +1,5 @@
 theory Bucket_Hash
-  imports PhiEx_Linked_Lst PhiEx_Rational PhiEx_DynArr
+  imports PhiEx_Linked_Lst PhiEx_Rational Dyn_Arr_arbi
 begin
 
 abbreviation \<open>\<k>\<v>_\<e>\<n>\<t>\<r>\<y> \<equiv> \<s>\<t>\<r>\<u>\<c>\<t>{k: \<a>\<i>\<n>\<t>, v: \<r>\<a>\<t>\<i>\<o>\<n>\<a>\<l>}\<close>
@@ -13,31 +13,30 @@ declare [[ML_print_depth = 1000]]
 lemma relational_functor_proof_obligation:
   \<open> \<forall>i<length xb. list_all2 (\<lambda>xa xy'. fst xy' = fst xa \<and> x (snd xa) (snd xy')) (xc i) (xd i)
 \<Longrightarrow> \<forall>i<length xb. list_all (\<lambda>(k, v). hash k (length xb) = i) (xc i) \<and> distinct (map fst (xc i))
-\<Longrightarrow> \<forall>k x. (xa k = Some x) = (\<exists>xa\<in>{..<length xb}. (k, x) \<in> set (xc xa))
+\<Longrightarrow> \<forall>k x. (xa k = Some x) = (\<exists>i<length xb. (k, x) \<in> set (xc i))
 \<Longrightarrow> \<exists>uu. (\<forall>i<length xb. list_all (\<lambda>(k, v). hash k (length xb) = i) (uu i) \<and> distinct (map fst (uu i))) \<and>
           (\<exists>uua. (\<forall>k x. (uua k = Some x) = (\<exists>i<length xb. (k, x) \<in> set (uu i))) \<and>
-                 dom xa = dom uua \<and>
-                 (\<forall>k\<in>dom uua. x (the (xa k)) (the (uua k))) \<and> (\<forall>i<length xb. list_all2 (\<lambda>x y. snd x = snd y \<and> fst x = fst y) (xd i) (uu i))) \<close>
+                 dom xa = dom uua \<and> (\<forall>k\<in>dom uua. x (the (xa k)) (the (uua k))) \<and> (\<forall>i<length xb. xd i = uu i)) \<close>
     apply (rule exI[where x=xd], auto simp: list_all2_conv_all_nth list_all_length)
-    apply fastforce
-    apply (metis (mono_tags, lifting) map_equality_iff)
+    apply auto_sledgehammer
+    apply auto_sledgehammer
     subgoal premises prems proof -
       have t1: \<open>\<forall>i<length xb. distinct (map fst (xd i))\<close>
-        by (smt (verit) map_equality_iff prems(1) prems(2))
+        by auto_sledgehammer
       have t2: \<open>\<exists>i<length xb. (k,v1) \<in> set (xd i)
             \<Longrightarrow> \<exists>i<length xb. (k,v2) \<in> set (xd i)
             \<Longrightarrow> v1 = v2\<close> for k v1 v2
         by (auto, smt (verit, ccfv_SIG) case_prod_beta' eq_key_imp_eq_value fst_conv last_index_less_size_conv local.t1 nth_last_index prems(1) prems(2))  
       have t3: \<open>(\<Union>i<length xb. set (xd i)) `` {k} = {} \<or> (\<exists>v. (\<Union>i<length xb. set (xd i)) `` {k} = {v})\<close> for k
-        by (insert t2, auto simp: set_eq_iff, metis lessThan_iff)
+        by (insert t2, auto simp: set_eq_iff, auto_sledgehammer)
       have t4: \<open>\<exists>g. \<forall>k x. g k = Some x \<longleftrightarrow> (\<exists>i<length xb. (k,x) \<in> set (xd i))\<close>
-        by (subst choice_iff[symmetric], metis option.sel option.simps(3) t2)
+        by (subst choice_iff[symmetric], auto_sledgehammer)
 
       have t5[simp]: \<open>xa k = Some y \<longleftrightarrow> (\<exists>i<length xb. (k,y) \<in> set (xc i))\<close> for k y
-        using prems(3) by auto
+        by auto_sledgehammer
 
       obtain g where g: \<open>\<forall>k x. g k = Some x \<longleftrightarrow> (\<exists>i<length xb. (k,x) \<in> set (xd i))\<close> for k
-        using t4 by blast
+        by auto_sledgehammer
 
       show ?thesis
         apply (rule exI[where x=g], auto simp: g)
@@ -50,12 +49,76 @@ qed .
 abbreviation \<open>\<h>\<a>\<s>\<h> \<equiv> \<s>\<t>\<r>\<u>\<c>\<t> {tabl: \<p>\<t>\<r>, N: \<a>\<i>\<n>\<t>} \<close>
 
 
+(*
+\<phi>type_def Bucket :: \<open>logaddr \<Rightarrow> nat \<Rightarrow> TY \<Rightarrow> (VAL, 'x) \<phi> \<Rightarrow> (fiction, 'x list) \<phi>\<close>
+  where \<open>bucket \<Ztypecolon> Bucket base i TY T \<equiv> ptr \<Ztypecolon> \<m>\<e>\<m>[base \<tribullet>\<^sub>a i\<^sup>\<t>\<^sup>\<h>] (\<Pp>\<t>\<r> \<l>\<i>\<n>\<k>_\<l>\<i>\<s>\<t> TY)\<heavy_comma>
+                                       bucket \<Ztypecolon> Linked_Lst ptr TY T
+                                       \<s>\<u>\<b>\<j> ptr. \<top>\<close>
+  deriving \<open> Abstract_Domain T P
+         \<Longrightarrow> Abstract_Domain (Bucket base i TY T) (list_all P)\<close>
+       and \<open> Object_Equiv T eq
+         \<Longrightarrow> Object_Equiv (Bucket base i TY T) (list_all2 eq) \<close>
+       and \<open> Transformation_Functor (Bucket base i TY) (Bucket base i TY) T U set (\<lambda>_. UNIV) list_all2 \<close>
+       and \<open> Functional_Transformation_Functor
+                (Bucket base i TY) (Bucket base i TY) T U set (\<lambda>_. UNIV)
+                (\<lambda>f P. list_all P) (\<lambda>f P. map f)\<close>  
+
+
+term \<open> Functional_Transformation_Functor
+                (Bucket base i) (Bucket base i) T U (\<lambda>x. snd ` set x) (\<lambda>_. UNIV)
+                (\<lambda>f P. list_all (P o snd)) (\<lambda>f P. map (apsnd f))\<close>
+
+
+
+
 \<phi>type_def Hash :: \<open>logaddr \<Rightarrow> (VAL, 'x) \<phi> \<Rightarrow> (fiction, nat \<rightharpoonup> 'x) \<phi>\<close>
   where \<open>f \<Ztypecolon> Hash addr T \<equiv> 
-       (tabl_addr, N) \<Ztypecolon> \<m>\<e>\<m>[addr] \<lbrace> tabl: \<Pp>\<t>\<r> \<a>\<r>\<r>\<a>\<y>[N] \<p>\<t>\<r>, N: \<nat> \<rbrace>\<heavy_comma>
+       (base, N) \<Ztypecolon> \<m>\<e>\<m>[addr] \<lbrace> tabl: \<Pp>\<t>\<r> \<a>\<r>\<r>\<a>\<y>[N] \<p>\<t>\<r>, N: \<nat> \<rbrace>\<heavy_comma>
+       buckets \<Ztypecolon> \<big_ast>\<^sup>\<phi> {i. i < N} (\<lambda>i. Bucket base i \<k>\<v>_\<e>\<n>\<t>\<r>\<y> \<lbrace>k: \<nat>, v: T\<rbrace>)
+       \<s>\<u>\<b>\<j> buckets base N.
+          (\<forall>i < N. list_all (\<lambda>(k,v). hash k N = i) (buckets i) \<and> distinct (map fst (buckets i))) \<and>
+          (\<forall>k x. f k = Some x \<longleftrightarrow> (\<exists>i<N. (k,x) \<in> set (buckets i))) \<and>
+          0 < N \<close>
+
+deriving \<open> Abstract_Domain T P
+         \<Longrightarrow> Abstract_Domain (Hash addr T) (\<lambda>f. \<forall>k \<in> dom f. P (the (f k)))\<close>
+    notes list_all_length[simp] Let_def[simp] set_eq_iff[simp]
+
+and \<open>Object_Equiv T eq
+    \<Longrightarrow> Object_Equiv (Hash addr T) (\<lambda>f g. dom f = dom g \<and> (\<forall>k \<in> dom g. eq (the (f k)) (the (g k))))\<close>
+   notes case_prod_beta[simp] list_all2_conv_all_nth[\<phi>sledgehammer_simps] list_all_length[\<phi>sledgehammer_simps]
+          image_iff[simp]
+    (tactic: auto simp: Ball_def Bex_def set_eq_iff,
+        subgoal' for f f' buckets tabl_addr \<open>rule exI[where x=\<open>\<lambda>i. map (\<lambda>(k,_). (k, the (f' k))) (buckets i)\<close>]\<close>,
+        auto_sledgehammer)
+
+(*
+and \<open>Transformation_Functor (Hash addr) (Hash addr) T U ran (\<lambda>_. UNIV) (\<lambda>r f g. dom f = dom g \<and> (\<forall>k \<in> dom g. r (the (f k)) (the (g k))))\<close>
+    notes set_eq_iff [\<phi>sledgehammer_simps]
+    (tactic: auto, auto_sledgehammer, tactic \<open>all_tac o @{print}\<close>, rule relational_functor_proof_obligation) 
+
+and \<open>Functional_Transformation_Functor (Hash addr) (Hash addr) T U ran (\<lambda>_. UNIV)
+          (\<lambda>_ P f. \<forall>k\<in>dom f. P (the (f k))) (\<lambda>h _ f. map_option h o f)\<close>
+*)
+
+
+*)
+
+
+
+
+
+
+
+
+
+
+\<phi>type_def Hash :: \<open>logaddr \<Rightarrow> (VAL, 'x) \<phi> \<Rightarrow> (fiction, nat \<rightharpoonup> 'x) \<phi>\<close>
+  where \<open>f \<Ztypecolon> Hash addr T \<equiv> 
+       buckets \<Ztypecolon> \<big_ast>\<^sup>\<phi> {i. i < N} (\<lambda>i.
+                  Linked_Lst (bucket_ptrs ! i) \<k>\<v>_\<e>\<n>\<t>\<r>\<y> \<lbrace>k: \<nat>, v: T\<rbrace>)\<heavy_comma>
        bucket_ptrs \<Ztypecolon> \<m>\<e>\<m>[tabl_addr] \<Aa>\<r>\<r>\<a>\<y>[N] (\<Pp>\<t>\<r> \<l>\<i>\<n>\<k>_\<l>\<i>\<s>\<t> \<k>\<v>_\<e>\<n>\<t>\<r>\<y>)\<heavy_comma>
-       buckets \<Ztypecolon> \<big_ast>\<^sup>\<phi> {i. i < length bucket_ptrs} (\<lambda>i.
-                  Linked_Lst (bucket_ptrs ! i) \<k>\<v>_\<e>\<n>\<t>\<r>\<y> \<lbrace>k: \<nat>, v: T\<rbrace>)
+       (tabl_addr, N) \<Ztypecolon> \<m>\<e>\<m>[addr] \<lbrace> tabl: \<Pp>\<t>\<r> \<a>\<r>\<r>\<a>\<y>[N] \<p>\<t>\<r>, N: \<nat> \<rbrace>
        \<s>\<u>\<b>\<j> bucket_ptrs buckets tabl_addr N.
           length bucket_ptrs = N \<and>
           (\<forall>i < N. list_all (\<lambda>(k,v). hash k N = i) (buckets i) \<and> distinct (map fst (buckets i))) \<and>
@@ -69,37 +132,101 @@ deriving \<open> Abstract_Domain T P
 and \<open>Object_Equiv T eq
     \<Longrightarrow> Object_Equiv (Hash addr T) (\<lambda>f g. dom f = dom g \<and> (\<forall>k \<in> dom g. eq (the (f k)) (the (g k))))\<close>
     notes case_prod_beta[simp] list_all2_conv_all_nth[\<phi>sledgehammer_simps] list_all_length[\<phi>sledgehammer_simps]
-          image_iff[simp]
+          image_iff[simp] domIff[simp]
     (tactic: auto simp: Ball_def Bex_def set_eq_iff,
         subgoal' for f f' xb buckets tabl_addr \<open>rule exI[where x=\<open>\<lambda>i. map (\<lambda>(k,_). (k, the (f' k))) (buckets i)\<close>]\<close> )
 
 and \<open>Transformation_Functor (Hash addr) (Hash addr) T U ran (\<lambda>_. UNIV) (\<lambda>r f g. dom f = dom g \<and> (\<forall>k \<in> dom g. r (the (f k)) (the (g k))))\<close>
     notes set_eq_iff [\<phi>sledgehammer_simps]
-    (tactic: auto, auto_sledgehammer, rule relational_functor_proof_obligation) 
+    (tactic: auto, auto_sledgehammer, tactic \<open>all_tac o @{print}\<close>, rule relational_functor_proof_obligation) 
 
 and \<open>Functional_Transformation_Functor (Hash addr) (Hash addr) T U ran (\<lambda>_. UNIV)
           (\<lambda>_ P f. \<forall>k\<in>dom f. P (the (f k))) (\<lambda>h _ f. map_option h o f)\<close>
 
 
-term \<open>f(a \<mapsto> b)\<close>
 
-declare Suc_le_eq[simp]
+context
+  fixes T :: \<open>(VAL, 'x) \<phi>\<close>
+    and zero :: 'x
+  assumes [\<phi>reason add]: \<open>\<phi>SemType (x \<Ztypecolon> T) \<r>\<a>\<t>\<i>\<o>\<n>\<a>\<l>\<close>
+      and [\<phi>reason add]: \<open>Semantic_Zero_Val \<r>\<a>\<t>\<i>\<o>\<n>\<a>\<l> T zero\<close>
+begin
 
-term \<open>S \<union> (D::'a set)\<close>
-term \<open>r |` S\<close>
+
+
+
+
+(*
+
+proc insert_bucket:
+  input \<open>bucket \<Ztypecolon> DynArr addr \<k>\<v>_\<e>\<n>\<t>\<r>\<y> \<lbrace> k: \<nat>, v: T \<rbrace>\<heavy_comma>
+         addr \<Ztypecolon> \<v>\<a>\<l> \<Pp>\<t>\<r> \<d>\<y>\<n>\<a>\<r>\<r>\<heavy_comma> k \<Ztypecolon> \<v>\<a>\<l> \<nat>\<heavy_comma> v \<Ztypecolon> \<v>\<a>\<l> T\<close>
+  premises \<open>distinct (map fst bucket)\<close>
+  output \<open>bucket' \<Ztypecolon> DynArr addr \<k>\<v>_\<e>\<n>\<t>\<r>\<y> \<lbrace> k: \<nat>, v: T \<rbrace>
+          \<s>\<u>\<b>\<j> bucket'. set bucket' = (set bucket - {(k',_). k' = k}) \<union> {(k,v)} \<and>
+                        distinct (map fst bucket') \<close>
+  is [recursive]
+  is [routine]
+\<medium_left_bracket>
+  var met \<leftarrow> False ;;
+  replicate_a (\<open>0 \<Ztypecolon> \<nat>\<close>, len_dynarr ($addr))
+              \<open>\<lambda>i. (map (\<lambda>kv. if fst kv = k then (k,v) else kv) (take i bucket) @ drop i bucket)
+                      \<Ztypecolon> DynArr addr \<k>\<v>_\<e>\<n>\<t>\<r>\<y> \<lbrace> k: \<nat>, v: T \<rbrace>\<heavy_comma>
+                   (\<exists>v. (k,v) \<in> set (take i bucket)) \<Ztypecolon> \<v>\<a>\<r>[met] \<bool>\<close>
+  \<medium_left_bracket> \<rightarrow> val i ;;
+    val kv \<leftarrow> get_dynarr($addr, $i) ;;
+    if ($kv \<tribullet> k = $k) \<medium_left_bracket>
+      set_dynarr($addr, $i, \<lbrace> k: $k, v: $v \<rbrace>) ;;
+      $met \<leftarrow> True
+    \<medium_right_bracket> \<medium_left_bracket> \<medium_right_bracket>
+  \<medium_right_bracket> certified by (auto simp add: list_eq_iff_nth_eq nth_append list_update_append; auto_sledgehammer) ;;
+  
+  if ($met) \<medium_left_bracket> \<medium_right_bracket> \<medium_left_bracket>
+    push_dynarr ($addr, \<lbrace> k: $k, v: $v \<rbrace>)
+  \<medium_right_bracket>
+\<medium_right_bracket> .
+
+*)
+
+
+
+
+
+
+
 
 proc insert_bucket:
   input \<open>bucket \<Ztypecolon> Linked_Lst addr \<k>\<v>_\<e>\<n>\<t>\<r>\<y> \<lbrace> k: \<nat>, v: T \<rbrace>\<heavy_comma>
-         addr \<Ztypecolon> \<v>\<a>\<l> \<Pp>\<t>\<r> \<l>\<i>\<n>\<k>_\<l>\<i>\<s>\<t> \<k>\<v>_\<e>\<n>\<t>\<r>\<y>\<heavy_comma> kk \<Ztypecolon> \<v>\<a>\<l> \<nat>\<heavy_comma> vv \<Ztypecolon> \<v>\<a>\<l> T\<close>
-  output \<open>bucket' \<Ztypecolon> Linked_Lst addr' \<k>\<v>_\<e>\<n>\<t>\<r>\<y> \<lbrace> k: \<nat>, v: T \<rbrace>
-          \<s>\<u>\<b>\<j> bucket' addr'. set bucket' = (set bucket - {(k',_). k' = k}) \<union> {(k,v)}\<close>
+         addr \<Ztypecolon> \<v>\<a>\<l> \<Pp>\<t>\<r> \<l>\<i>\<n>\<k>_\<l>\<i>\<s>\<t> \<k>\<v>_\<e>\<n>\<t>\<r>\<y>\<heavy_comma> k \<Ztypecolon> \<v>\<a>\<l> \<nat>\<heavy_comma> v \<Ztypecolon> \<v>\<a>\<l> T\<close>
+  premises \<open>distinct (map fst bucket)\<close>
+  output \<open>bucket' \<Ztypecolon> Linked_Lst addr' \<k>\<v>_\<e>\<n>\<t>\<r>\<y> \<lbrace> k: \<nat>, v: T \<rbrace>\<heavy_comma>
+          addr' \<Ztypecolon> \<v>\<a>\<l> \<Pp>\<t>\<r> \<l>\<i>\<n>\<k>_\<l>\<i>\<s>\<t> \<k>\<v>_\<e>\<n>\<t>\<r>\<y>
+          \<s>\<u>\<b>\<j> bucket' addr'. set bucket' = (set bucket - {(k',_). k' = k}) \<union> {(k,v)} \<and>
+                             distinct (map fst bucket') \<close>
+  is [recursive]
+  is [routine]
 \<medium_left_bracket>
   if \<open>$addr = 0\<close> \<medium_left_bracket>   
-    \<lbrace> k: $kk, v: $vv \<rbrace>
+    val ret \<leftarrow> prepend_llist ($addr, \<lbrace> k: $k, v: $v \<rbrace>) ;;
+    return ($ret)
+  \<medium_right_bracket> \<medium_left_bracket>
+    to \<open>OPEN 1 _\<close> ;;
+    if ($addr \<tribullet> data \<tribullet> k! = $k) \<medium_left_bracket>
+      $addr \<tribullet> data \<tribullet> v := $v ;;
+      \<open>MAKE 1 (Linked_Lst addr _ _)\<close> ;;
+      return ($addr) (* certified by (simp, rule exI[where x=\<open>(k, v) # tl bucket\<close>], auto_sledgehammer) *)
+    \<medium_right_bracket> \<medium_left_bracket>
+      val addr' \<leftarrow> insert_bucket ($addr \<tribullet> nxt!, $k, $v) ;;
+      $addr \<tribullet> nxt := $addr' ;;
+      \<open>MAKE 1 (Linked_Lst addr _ _)\<close> ;;
+      return ($addr)
+    \<medium_right_bracket>
+  \<medium_right_bracket>   
+\<medium_right_bracket> .
 (*    prepend_llist ($addr,  *)
 
 
-
+declare Suc_le_eq[simp]
 
 proc update_hash:
   input  \<open>f \<Ztypecolon> Hash addr T\<heavy_comma> addr \<Ztypecolon> \<v>\<a>\<l> \<Pp>\<t>\<r> \<h>\<a>\<s>\<h>\<heavy_comma> k \<Ztypecolon> \<v>\<a>\<l> \<nat>\<heavy_comma> v \<Ztypecolon> \<v>\<a>\<l> T\<close>
@@ -109,11 +236,41 @@ proc update_hash:
   val tabl_addr \<leftarrow> $addr \<tribullet> tabl ! \<semicolon>
   val N \<leftarrow> $addr \<tribullet> N ! \<semicolon>
   val hash \<leftarrow> $k % $N \<semicolon>
-  $tabl_addr \<tribullet> $hash !
+  val new_bucket \<leftarrow> insert_bucket ($tabl_addr \<tribullet> $hash !, $k, $v) \<semicolon>
+  $tabl_addr \<tribullet> $hash := $new_bucket ;;
+
+  define bucket_ptrs' where t1: \<open>bucket_ptrs' \<equiv> list_upd_map (hash k (length bucket_ptrs)) (comb.K addr') bucket_ptrs\<close>
+  note t1[symmetric, simp] ;;
+  holds_fact t2[simp]: \<open>length bucket_ptrs = length bucket_ptrs' \<and>
+                        addr' = bucket_ptrs' ! (hash k (length bucket_ptrs')) \<close> ;;
+  holds_fact [simp]:
+       \<open> \<big_ast>\<^sup>\<phi> ({i. i < length bucket_ptrs'} - {hash k (length bucket_ptrs')}) (\<lambda>i. Linked_Lst (bucket_ptrs ! i) \<k>\<v>_\<e>\<n>\<t>\<r>\<y> \<lbrace> k: \<nat>, v: T \<rbrace>)
+       = \<big_ast>\<^sup>\<phi> ({i. i < length bucket_ptrs'} - {hash k (length bucket_ptrs')}) (\<lambda>i. Linked_Lst (bucket_ptrs' ! i) \<k>\<v>_\<e>\<n>\<t>\<r>\<y> \<lbrace> k: \<nat>, v: T \<rbrace>) \<close>  ;;
+
+  holds_fact [\<phi>safe_simp]:
+    \<open>{i. i < length bucket_ptrs'} - ({i. i < length bucket_ptrs'} - {hash k (length bucket_ptrs')}) = {hash k (length bucket_ptrs')}\<close> ;;
+  \<open>_ \<Ztypecolon> \<big_ast>\<^sup>\<phi> ({i. i < length bucket_ptrs'} - {hash k (length bucket_ptrs')}) (\<lambda>i. Linked_Lst (bucket_ptrs' ! i) \<k>\<v>_\<e>\<n>\<t>\<r>\<y> \<lbrace> k: \<nat>, v: T \<rbrace>) \<close> ;;
+  \<open>_ \<Ztypecolon> \<big_ast>\<^sup>\<phi> ({i. i < length bucket_ptrs'}) (\<lambda>i. Linked_Lst (bucket_ptrs' ! i) \<k>\<v>_\<e>\<n>\<t>\<r>\<y> \<lbrace> k: \<nat>, v: T \<rbrace>) \<close> ;;
 
 
-thm mod_\<phi>app
-
+  \<open>f(k \<mapsto> v) \<Ztypecolon> MAKE _ (Hash addr T)\<close> certified apply (auto, auto_sledgehammer)
+      apply (rule exI[where x=\<open>\<lambda>i. if i = hash k (length bucket_ptrs') then bucket' else buckets i\<close>])
+      apply (clarsimp simp: list_all2_conv_all_nth list_all_length)
+      subgoal premises prems
+      proof -
+        note [\<phi>sledgehammer_simps] = list_all2_conv_all_nth list_all_length
+        let ?N = \<open>length bucket_ptrs'\<close>
+        have t1: \<open> \<lbrakk> (k',v) \<in> set bucket' ; k' \<noteq> k \<rbrakk> \<Longrightarrow> (k', v) \<in> set (buckets (hash k ?N)) \<close> for n k' v
+          by auto_sledgehammer
+        have t2: \<open>\<lbrakk> (k,v) \<in> set (buckets i) ; i < ?N \<rbrakk> \<Longrightarrow> hash k ?N = i\<close> for k v i 
+          by auto_sledgehammer
+        show ?thesis
+          apply (auto, metis local.t1 nth_mem t2)
+          apply (metis \<open>list_upd_map (hash k (length bucket_ptrs)) (comb.K addr') bucket_ptrs \<equiv> bucket_ptrs'\<close> bot_nat_0.not_eq_extremum length_0_conv length_list_upd_map mod_less_divisor the_\<phi>lemmata(6))
+          using t2 apply blast
+          by metis
+        qed .
+\<medium_right_bracket> .
 
 
 end
